Source/Dafny/AST/TokenFormatter.dfy
@@ -1,37 +1,34 @@
-module {:extern @" Helpers {
-  public class HelperString {
-    public static readonly System.Text.RegularExpressions.Regex NewlineRegex =
-      new System.Text.RegularExpressions.Regex(new string(new char[]  
-        {'(','?','m',')','(','^',')','\\','s','*'}));
-
-    public static string Reindent(string input, string newIndent) {
-      return NewlineRegex.Replace(input, newIndent);
-    }
+module {:extern @"Microsoft.Dafny.Helpers"} {:options "-functionSyntax:4"} Helpers {
+  import opened System
+  class {:extern "HelperString"} {:compile false} HelperString {
+    static function Reindent(input: CsString, indentationBefore: CsString, lastIndentation: CsString): CsString
   }
-} /*/"} DefaultCode {
 }
 module {:extern "System"} {:compile false} {:options "-functionSyntax:4"} System {
-  type {:extern "String"} CsString(!new)
+  type {:extern "String"} CsString(!new) {
+    function Length(): int
+  }
   class {:extern "String"} {:compile false} String {
-    static function Concat(s1: CsString, s2: CsString): CsString
+    static function Concat(s1: CsString, s2: CsString): (r: CsString)
+      ensures r.Length() >= s1.Length()
+      ensures r.Length() >= s2.Length()
   }
 }
-module {:extern "/*/dummy{}", "Top"} {:compile false} {:options "-functionSyntax:4"} Top {
+module {:extern "Microsoft.Dafny"} {:compile false} {:options "-functionSyntax:4"} MicrosoftDafny {
   import opened System
-  trait {:extern "*/Microsoft.Dafny.IToken"} {:compile false} IToken {
+  trait {:extern "IToken"} {:compile false} IToken {
     var val: CsString
     var LeadingTrivia: CsString
     var TrailingTrivia: CsString
-    ghost var remainingTokens: seq<IToken>
+    ghost var remainingTokens: nat
     var Next: IToken?
 
-    ghost predicate Valid() reads * decreases |remainingTokens| {
+    ghost predicate Valid() reads * decreases remainingTokens {
       if Next == null then
-        remainingTokens == []
+        remainingTokens == 0
       else
-        && |remainingTokens| > 0
-        && Next == remainingTokens[0]
-        && Next.remainingTokens == remainingTokens[1..]
+        && remainingTokens > 0
+        && Next.remainingTokens == remainingTokens - 1
         && Next.Valid()
     }
   }
@@ -39,8 +36,9 @@ module {:extern "/*/dummy{}", "Top"} {:compile false} {:options "-functionSyntax
 module {:extern "Microsoft"} {:options "-functionSyntax:4"}  Microsoft {
   module {:extern "Dafny"} Dafny {
     module {:extern "TokenFormatter"} TokenFormatter {
-      import opened Top
+      import opened MicrosoftDafny
       import opened System
+      import opened Helpers
 
       newtype {:native} CInt = x: int | 0 <= x < 65535
 
@@ -48,11 +46,14 @@ module {:extern "Microsoft"} {:options "-functionSyntax:4"}  Microsoft {
       function {:extern} {:macro "new string(character, length)"} newString(character: char, length: CInt): CsString
       const {:extern "System", "String.Empty"} CsStringEmpty: CsString;
 
-      function {:extern "Helpers.HelperString", "Reindent"} {:macro} Reindent(input: CsString, newIndent: CsString): (output: CsString)
-
       trait ITokenIndentations {
         // Returns -1 if no indentation is set
-        method getIndentation(token: IToken) returns (indentation: CsString, wasSet: bool)
+        method GetIndentation(token: IToken, currentIndentation: CsString)
+          returns (
+            indentationBefore: CsString,
+            lastIndentation: CsString,
+            indentationAfter: CsString,
+            wasSet: bool)
       }
       
       
@@ -64,8 +65,8 @@ module {:extern "Microsoft"} {:options "-functionSyntax:4"}  Microsoft {
         var token: IToken? := firstToken;
         s := CsStringEmpty;
         while(token != null)
-        decreases if token == null then 0 else |token.remainingTokens| + 1
-        invariant token == null || token.Valid()
+          decreases if token == null then 0 else token.remainingTokens + 1
+          invariant token == null || token.Valid()
         {
           s := String.Concat(String.Concat(String.Concat(s, token.LeadingTrivia), token.val), token.TrailingTrivia);
           token := token.Next;
@@ -79,21 +80,36 @@ module {:extern "Microsoft"} {:options "-functionSyntax:4"}  Microsoft {
         var token: IToken? := firstToken;
         s := CsStringEmpty;
         var currentIndent := CsStringEmpty;
+        var currentIndentLast := CsStringEmpty;
         var isSet := false;
+        var previousTrailingTrivia := CsStringEmpty;
+        ghost var sLengthPrev := s.Length();
         while(token != null)
-        decreases if token == null then 0 else |token.remainingTokens| + 1
+        decreases if token == null then 0 else token.remainingTokens + 1
         invariant token == null || token.Valid()
+        invariant sLengthPrev <= s.Length();
         {
-          var newIndent, wasSet := reindent.getIndentation(token);
+          sLengthPrev := s.Length();
+          var indentationBefore, lastIndentation, indentationAfter, wasSet := reindent.GetIndentation(token, currentIndent);
           if(wasSet) {
-            currentIndent := newIndent;
+            currentIndent := indentationBefore;
+            currentIndentLast := lastIndentation;
             isSet := true;
           }
-          var LeadingTrivia := if isSet then Reindent(token.LeadingTrivia, currentIndent) else token.LeadingTrivia;
-          var TrailingTrivia :=  if isSet then Reindent(token.TrailingTrivia, newIndent) else token.TrailingTrivia;
-          s := String.Concat(String.Concat(String.Concat(s, LeadingTrivia), token.val), TrailingTrivia);
+          var triviaSoFar := String.Concat(previousTrailingTrivia, token.LeadingTrivia);
+          var newTrivia := if isSet then
+            HelperString.Reindent(triviaSoFar, indentationBefore, lastIndentation) else triviaSoFar;
+          // Had an error here: caught by an invariant
+          //s := String.Concat(newTrivia, token.val);
+          s := String.Concat(s, String.Concat(newTrivia, token.val));
+          previousTrailingTrivia := token.TrailingTrivia;
+          if(wasSet) {
+            currentIndent := indentationAfter;
+          }
+
           token := token.Next;
         }
+        s := String.Concat(s, previousTrailingTrivia);
       }
     }
   }
